P9: add sar64 + sar32 (signed arithmetic right shift, 2 hits)
Includes signedShiftRight64/signedShiftRight32 helper functions
in VexSyntax.lean. SMT uses bvashr.

Instances/ISAs/AntiUnify.lean
@@ -67,6 +67,8 @@ inductive TemplateExpr (Reg : Type) where
   | mul32 : TemplateExpr Reg → TemplateExpr Reg → TemplateExpr Reg
   | not64 : TemplateExpr Reg → TemplateExpr Reg
   | not32 : TemplateExpr Reg → TemplateExpr Reg
+  | sar64 : TemplateExpr Reg → TemplateExpr Reg → TemplateExpr Reg
+  | sar32 : TemplateExpr Reg → TemplateExpr Reg → TemplateExpr Reg
   | load : Width → TemplateMem Reg → TemplateExpr Reg → TemplateExpr Reg
 
 /-- A template memory: like SymMem but expressions may have holes.
@@ -108,6 +110,8 @@ def embedExpr {Reg : Type} : SymExpr Reg → TemplateExpr Reg
   | .sext32to64 x => .sext32to64 (embedExpr x)
   | .not64 x => .not64 (embedExpr x)
   | .not32 x => .not32 (embedExpr x)
+  | .sar64 a b => .sar64 (embedExpr a) (embedExpr b)
+  | .sar32 a b => .sar32 (embedExpr a) (embedExpr b)
   | .sub32 a b => .sub32 (embedExpr a) (embedExpr b)
   | .and32 a b => .and32 (embedExpr a) (embedExpr b)
   | .or32 a b => .or32 (embedExpr a) (embedExpr b)
@@ -278,6 +282,7 @@ def TemplateExpr.holeCount {Reg : Type} : TemplateExpr Reg → Nat
   | .hole _ => 1
   | .const _ | .reg _ => 0
   | .low32 x | .uext32 x | .sext8to32 x | .sext32to64 x | .not64 x | .not32 x => x.holeCount
+  | .sar64 a b | .sar32 a b => a.holeCount + b.holeCount
   | .sub32 a b | .shl32 a b | .and32 a b | .or32 a b | .xor32 a b | .add64 a b | .sub64 a b
   | .xor64 a b | .and64 a b | .or64 a b | .shl64 a b | .shr64 a b | .mul64 a b | .mul32 a b =>
     a.holeCount + b.holeCount
@@ -314,6 +319,8 @@ def instantiateExpr {Reg : Type} (val : HoleVal Reg) : TemplateExpr Reg → SymE
   | .sext32to64 x => .sext32to64 (instantiateExpr val x)
   | .not64 x => .not64 (instantiateExpr val x)
   | .not32 x => .not32 (instantiateExpr val x)
+  | .sar64 a b => .sar64 (instantiateExpr val a) (instantiateExpr val b)
+  | .sar32 a b => .sar32 (instantiateExpr val a) (instantiateExpr val b)
   | .sub32 a b => .sub32 (instantiateExpr val a) (instantiateExpr val b)
   | .and32 a b => .and32 (instantiateExpr val a) (instantiateExpr val b)
   | .or32 a b => .or32 (instantiateExpr val a) (instantiateExpr val b)
@@ -362,6 +369,8 @@ theorem instantiateExpr_embedExpr {Reg : Type} (val : HoleVal Reg) (e : SymExpr 
   | .sext32to64 x => simp [embedExpr, instantiateExpr, instantiateExpr_embedExpr val x]
   | .not64 x => simp [embedExpr, instantiateExpr, instantiateExpr_embedExpr val x]
   | .not32 x => simp [embedExpr, instantiateExpr, instantiateExpr_embedExpr val x]
+  | .sar64 a b => simp [embedExpr, instantiateExpr, instantiateExpr_embedExpr val a, instantiateExpr_embedExpr val b]
+  | .sar32 a b => simp [embedExpr, instantiateExpr, instantiateExpr_embedExpr val a, instantiateExpr_embedExpr val b]
   | .sub32 a b => simp [embedExpr, instantiateExpr, instantiateExpr_embedExpr val a, instantiateExpr_embedExpr val b]
   | .and32 a b => simp [embedExpr, instantiateExpr, instantiateExpr_embedExpr val a, instantiateExpr_embedExpr val b]  | .shl32 a b => simp [embedExpr, instantiateExpr, instantiateExpr_embedExpr val a, instantiateExpr_embedExpr val b]
   | .or32 a b => simp [embedExpr, instantiateExpr, instantiateExpr_embedExpr val a, instantiateExpr_embedExpr val b]
@@ -472,6 +481,7 @@ def TemplateExpr.holesBelow {Reg : Type} (n : Nat) : TemplateExpr Reg → Prop
   | .hole h => h < n
   | .const _ | .reg _ => True
   | .low32 x | .uext32 x | .sext8to32 x | .sext32to64 x | .not64 x | .not32 x => x.holesBelow n
+  | .sar64 a b | .sar32 a b => a.holesBelow n ∧ b.holesBelow n
   | .sub32 a b | .shl32 a b | .and32 a b | .or32 a b | .xor32 a b | .add64 a b | .sub64 a b
   | .xor64 a b | .and64 a b | .or64 a b | .shl64 a b | .shr64 a b | .mul64 a b | .mul32 a b =>
     a.holesBelow n ∧ b.holesBelow n
@@ -500,6 +510,8 @@ theorem embedExpr_holesBelow {Reg : Type} (e : SymExpr Reg) (n : Nat) :
   | .sext32to64 x => exact embedExpr_holesBelow x n
   | .not64 x => exact embedExpr_holesBelow x n
   | .not32 x => exact embedExpr_holesBelow x n
+  | .sar64 a b => exact ⟨embedExpr_holesBelow a n, embedExpr_holesBelow b n⟩
+  | .sar32 a b => exact ⟨embedExpr_holesBelow a n, embedExpr_holesBelow b n⟩
   | .sub32 a b => exact ⟨embedExpr_holesBelow a n, embedExpr_holesBelow b n⟩
   | .and32 a b => exact ⟨embedExpr_holesBelow a n, embedExpr_holesBelow b n⟩  | .shl32 a b => exact ⟨embedExpr_holesBelow a n, embedExpr_holesBelow b n⟩
   | .or32 a b => exact ⟨embedExpr_holesBelow a n, embedExpr_holesBelow b n⟩
@@ -556,6 +568,14 @@ theorem instantiateExpr_val_agree {Reg : Type} {n : Nat}
     simp [instantiateExpr]; exact instantiateExpr_val_agree x h_below h_agree
   | .not32 x =>
     simp [instantiateExpr]; exact instantiateExpr_val_agree x h_below h_agree
+  | .sar64 a b =>
+    simp [instantiateExpr]
+    exact ⟨instantiateExpr_val_agree a h_below.1 h_agree,
+           instantiateExpr_val_agree b h_below.2 h_agree⟩
+  | .sar32 a b =>
+    simp [instantiateExpr]
+    exact ⟨instantiateExpr_val_agree a h_below.1 h_agree,
+           instantiateExpr_val_agree b h_below.2 h_agree⟩
   | .sub32 a b =>
     simp [instantiateExpr]
     exact ⟨instantiateExpr_val_agree a h_below.1 h_agree,
@@ -812,6 +832,12 @@ theorem TemplateExpr.holesBelow_mono {Reg : Type} {n m : Nat}
   | .const _ | .reg _ => trivial
   | .low32 x | .uext32 x | .sext8to32 x | .sext32to64 x | .not64 x | .not32 x =>
     exact TemplateExpr.holesBelow_mono x h h_le
+  | .sar64 a b =>
+    exact ⟨TemplateExpr.holesBelow_mono a h.1 h_le,
+           TemplateExpr.holesBelow_mono b h.2 h_le⟩
+  | .sar32 a b =>
+    exact ⟨TemplateExpr.holesBelow_mono a h.1 h_le,
+           TemplateExpr.holesBelow_mono b h.2 h_le⟩
   | .sub32 a b | .shl32 a b | .and32 a b | .or32 a b | .xor32 a b | .add64 a b | .sub64 a b
   | .xor64 a b | .and64 a b | .or64 a b | .shl64 a b | .shr64 a b | .mul64 a b | .mul32 a b =>
     exact ⟨TemplateExpr.holesBelow_mono a h.1 h_le,
@@ -1330,6 +1356,8 @@ def substTemplateExpr {Reg : Type} [DecidableEq Reg] [Fintype Reg]
   | .sext32to64 x => .sext32to64 (substTemplateExpr σ x)
   | .not64 x => .not64 (substTemplateExpr σ x)
   | .not32 x => .not32 (substTemplateExpr σ x)
+  | .sar64 a b => .sar64 (substTemplateExpr σ a) (substTemplateExpr σ b)
+  | .sar32 a b => .sar32 (substTemplateExpr σ a) (substTemplateExpr σ b)
   | .sub32 a b => .sub32 (substTemplateExpr σ a) (substTemplateExpr σ b)
   | .and32 a b => .and32 (substTemplateExpr σ a) (substTemplateExpr σ b)
   | .or32 a b => .or32 (substTemplateExpr σ a) (substTemplateExpr σ b)
@@ -1395,6 +1423,8 @@ theorem embedExpr_substSymExpr {Reg : Type} [DecidableEq Reg] [Fintype Reg]
   | .sext32to64 x => simp [substSymExpr, embedExpr, substTemplateExpr, embedExpr_substSymExpr σ x]
   | .not64 x => simp [substSymExpr, embedExpr, substTemplateExpr, embedExpr_substSymExpr σ x]
   | .not32 x => simp [substSymExpr, embedExpr, substTemplateExpr, embedExpr_substSymExpr σ x]
+  | .sar64 a b => simp [substSymExpr, embedExpr, substTemplateExpr, embedExpr_substSymExpr σ a, embedExpr_substSymExpr σ b]
+  | .sar32 a b => simp [substSymExpr, embedExpr, substTemplateExpr, embedExpr_substSymExpr σ a, embedExpr_substSymExpr σ b]
   | .sub32 a b => simp [substSymExpr, embedExpr, substTemplateExpr, embedExpr_substSymExpr σ a, embedExpr_substSymExpr σ b]
   | .and32 a b => simp [substSymExpr, embedExpr, substTemplateExpr, embedExpr_substSymExpr σ a, embedExpr_substSymExpr σ b]  | .shl32 a b => simp [substSymExpr, embedExpr, substTemplateExpr, embedExpr_substSymExpr σ a, embedExpr_substSymExpr σ b]
   | .or32 a b => simp [substSymExpr, embedExpr, substTemplateExpr, embedExpr_substSymExpr σ a, embedExpr_substSymExpr σ b]
@@ -1440,6 +1470,8 @@ theorem substTemplateExpr_holesBelow {Reg : Type} [DecidableEq Reg] [Fintype Reg
   | .sext32to64 x => exact substTemplateExpr_holesBelow σ x n h
   | .not64 x => exact substTemplateExpr_holesBelow σ x n h
   | .not32 x => exact substTemplateExpr_holesBelow σ x n h
+  | .sar64 a b => exact ⟨substTemplateExpr_holesBelow σ a n h.1, substTemplateExpr_holesBelow σ b n h.2⟩
+  | .sar32 a b => exact ⟨substTemplateExpr_holesBelow σ a n h.1, substTemplateExpr_holesBelow σ b n h.2⟩
   | .sub32 a b => exact ⟨substTemplateExpr_holesBelow σ a n h.1, substTemplateExpr_holesBelow σ b n h.2⟩
   | .and32 a b => exact ⟨substTemplateExpr_holesBelow σ a n h.1, substTemplateExpr_holesBelow σ b n h.2⟩  | .shl32 a b => exact ⟨substTemplateExpr_holesBelow σ a n h.1, substTemplateExpr_holesBelow σ b n h.2⟩
   | .or32 a b => exact ⟨substTemplateExpr_holesBelow σ a n h.1, substTemplateExpr_holesBelow σ b n h.2⟩
@@ -1507,6 +1539,12 @@ theorem substSymExpr_instantiateExpr {Reg : Type} [DecidableEq Reg] [Fintype Reg
     simp [instantiateExpr, substSymExpr, substTemplateExpr, substSymExpr_instantiateExpr σ v x]
   | .not32 x =>
     simp [instantiateExpr, substSymExpr, substTemplateExpr, substSymExpr_instantiateExpr σ v x]
+  | .sar64 a b =>
+    simp [instantiateExpr, substSymExpr, substTemplateExpr,
+          substSymExpr_instantiateExpr σ v a, substSymExpr_instantiateExpr σ v b]
+  | .sar32 a b =>
+    simp [instantiateExpr, substSymExpr, substTemplateExpr,
+          substSymExpr_instantiateExpr σ v a, substSymExpr_instantiateExpr σ v b]
   | .sub32 a b =>
     simp [instantiateExpr, substSymExpr, substTemplateExpr,
           substSymExpr_instantiateExpr σ v a, substSymExpr_instantiateExpr σ v b]
